dpll_optimized/DpllPropagation.fst
@@ -52,7 +52,7 @@ let assign_literal_true_in_truth
     (t : truth_assignment) 
     ( l : literal{is_variable_in_assignment t (get_literal_variable l) = false})
     : (res : truth_assignment{
-        (forall (v : variable_info{L.mem v t}). (L.mem v res))
+        t1_is_sublist_of_t2 t res
         /\ length res = length t + 1
         /\ is_variable_in_assignment res (get_literal_variable l)
         /\ get_literal_value res l = true
@@ -110,206 +110,6 @@ let lemma_dpll_helper_1 (t : truth_assignment) ( c : clause) : Lemma
 let negate_var_info (v : variable_info) : (res :variable_info {res.value = not v.value /\ v.variable=res.variable})
     = {value = (not v.value) ; variable = v.variable}
 
-// let propagate_unit_clause_lemma_helper 
-//     (f : formula) 
-//     ( cl : clause) 
-//     (t: truth_assignment ) 
-//     (res : (truth_assignment * literal))
-//     : Lemma
-//     (requires 
-//         L.mem cl f
-//         /\ is_unit_clause cl t /\ no_variables_outside_f_are_in_t f t
-//         /\ (snd res) = (get_unassigned_literal_in_unit_clause cl t)
-//         /\ (fst res) = assign_literal_true_in_truth t (snd res) 
-//     )
-//     (ensures 
-//         is_unit_clause cl res._1 = false
-//         /\ is_clause_true_yet res._1 cl
-//         /\ (length res._1 = length t + 1)
-//         /\ (forall (v : variable_info{L.mem v t}). (L.mem v res._1)) 
-//         /\ no_variables_outside_f_are_in_t f res._1
-//         /\ (( forall (whole_t: truth_assignment{ 
-//                     (forall (v : variable_info {(List.Tot.mem v t)}). ((List.Tot.mem v whole_t)))
-//                     /\ are_variables_in_truth_assignment f whole_t 
-//                     /\ length whole_t =  length ( get_vars_in_formula f)}). 
-//                     (is_solution f whole_t = false)) 
-//                 <==> 
-//                 ( forall (whole_t: truth_assignment{ 
-//                     (forall (v : variable_info {(List.Tot.mem v res._1)}). ((List.Tot.mem v whole_t)))
-//                     /\ are_variables_in_truth_assignment f whole_t 
-//                     /\ length whole_t =  length ( get_vars_in_formula f)}). 
-//                     (is_solution f whole_t = false)) )
-
-//         /\ is_variable_in_assignment t (get_literal_variable res._2) = false
-//         /\ is_variable_in_assignment res._1 (get_literal_variable res._2)
-//         /\ is_lit_in_formula f res._2
-//         /\ (forall (l : literal {
-//                 is_variable_in_assignment res._1 (get_literal_variable l)
-//                 /\ (l <> (negate_lit res._2))
-//                 /\ (l <> res._2)}) . 
-//                     (is_variable_in_assignment t (get_literal_variable l)))
-        
-//         /\ (forall (l : literal {
-//                 is_variable_in_assignment t (get_literal_variable l)
-//             }). (get_literal_value t l = get_literal_value res._1 l)))
-//     = 
-//     let x = snd res in
-//     let x_variable = get_literal_variable x in
-//     let ress = fst res in
-//     let anti_res = assign_literal_true_in_truth t (negate_lit x) in
-//         assert((length (get_unassigned_literals_from_clause cl t) = 1) /\ (L.hd (get_unassigned_literals_from_clause cl t)) = x);
-//         assert(forall (n : nat_non_zero{ is_variable_in_assignment t n}). ( is_variable_in_assignment anti_res n));
-
-//         assert(forall (l : literal{L.mem l cl /\ l <> x}). (is_variable_in_assignment anti_res (get_literal_variable l)));
-//         assert(is_variable_in_assignment anti_res (get_literal_variable x));
-//         assert(forall (l : literal{L.mem l cl}). ((is_variable_in_assignment anti_res (get_literal_variable l)) ));
-//         assert(forall (l : literal{L.mem l cl}). ( (get_literal_value anti_res l = false)));
-
-//         assert(((are_clause_vars_in_assignment anti_res cl)));
-//         assert(forall (l : literal{L.mem l cl}). (get_literal_value anti_res l = false));
-//         assert(~(exists (l : literal{L.mem l cl}). (get_literal_value anti_res l)));
-//         assert((get_clause_value anti_res cl) <==> (exists (l : literal{L.mem l cl}). (get_literal_value anti_res l = true)));
-//         assert((~(exists (l : literal{L.mem l cl}). (get_literal_value anti_res l))) ==> (get_clause_value anti_res cl = false) );
-//         lemma_dpll_helper_1 anti_res cl;
-//         assert( get_clause_value anti_res cl = false) ;
-//         assert(is_clause_false_yet anti_res cl = true);
-//         assert(is_partial_solution f anti_res = false);
-
-//         let v1 = {value = Var? (get_unassigned_literal_in_unit_clause cl t) ; variable = (get_literal_variable (get_unassigned_literal_in_unit_clause cl t)) } in
-//         let v2 = negate_var_info v1 in
-
-//         assert(
-//             forall (other_t : truth_assignment {
-//                 (forall (v : variable_info{L.mem v anti_res}). (L.mem v other_t))}). 
-//                     (forall (l : literal{L.mem l cl}). (is_variable_in_assignment other_t (get_literal_variable l)))
-//         );
-//         assert(
-//             forall (other_t : truth_assignment {
-//                 (forall (v : variable_info{L.mem v anti_res}). (L.mem v other_t))}). 
-//                     (forall (l : literal{L.mem l cl}). (get_literal_value anti_res l = get_literal_value other_t l))
-//         );
-//         assert(
-//             forall (other_t : truth_assignment {
-//                 (forall (v : variable_info{L.mem v anti_res}). (L.mem v other_t))}). 
-//                     (get_clause_value anti_res cl = get_clause_value other_t cl)
-//         );
-//         assert( get_clause_value anti_res cl = false) ;
-//         assert(
-//             forall (other_t : truth_assignment {
-//                 (forall (v : variable_info{L.mem v anti_res}). (L.mem v other_t))}). 
-//                     (false = get_clause_value other_t cl)
-//         );
-//         assert(
-//             forall (other_t : truth_assignment {
-//                 (forall (v : variable_info{L.mem v anti_res}). (L.mem v other_t))}). 
-//                 (is_partial_solution f other_t = false)
-//         );
-
-//         assert(forall (other_t : truth_assignment {
-//             (forall (v : variable_info{L.mem v t}). (L.mem v other_t)) 
-//             /\ L.mem v2 other_t}). (is_partial_solution f other_t = false));
-
-//         assert(v2 = {value = Var? (negate_lit (get_unassigned_literal_in_unit_clause cl t)) ; variable = (get_literal_variable (get_unassigned_literal_in_unit_clause cl t)) });
-//         assert(L.mem v2 anti_res);
-//         assert(( forall (whole_t: truth_assignment{ 
-//                 (forall (v : variable_info {(List.Tot.mem v t)}). ((List.Tot.mem v whole_t)))
-//                 /\ are_variables_in_truth_assignment f whole_t 
-//                 /\ length whole_t =  length ( get_vars_in_formula f)}). 
-//                     (is_variable_in_assignment whole_t x_variable)));
-
-//         assert(( forall (whole_t: truth_assignment{ 
-//                 (forall (v : variable_info {(List.Tot.mem v t)}). ((List.Tot.mem v whole_t)))
-//                 /\ are_variables_in_truth_assignment f whole_t 
-//                 /\ length whole_t =  length ( get_vars_in_formula f)}). 
-//                    (L.mem v1 whole_t || L.mem v2 whole_t)));
-
-//         assert(( forall (whole_t: truth_assignment{ 
-//                 (forall (v : variable_info {(List.Tot.mem v t)}). ((List.Tot.mem v whole_t)))
-//                 /\ are_variables_in_truth_assignment f whole_t 
-//                 /\ length whole_t =  length ( get_vars_in_formula f)}). 
-//                    (L.mem v1 whole_t = not (L.mem v2 whole_t))));
-
-//         assert(( forall (whole_t: truth_assignment{ 
-//                 (forall (v : variable_info {(List.Tot.mem v t)}). ((List.Tot.mem v whole_t)))
-//                 /\ are_variables_in_truth_assignment f whole_t 
-//                 /\ L.mem v2 whole_t
-//                 /\ length whole_t =  length ( get_vars_in_formula f)}). 
-//                    (is_solution f whole_t = false)));
-
-//         assert(( forall (whole_t: truth_assignment{ 
-//                 (forall (v : variable_info {(List.Tot.mem v t)}). ((List.Tot.mem v whole_t)))
-//                 /\ are_variables_in_truth_assignment f whole_t 
-//                 /\ (exists (v : variable_info  {L.mem v ress}). (L.mem v whole_t = false))
-//                 /\ length whole_t =  length ( get_vars_in_formula f)}). 
-//                    (is_solution f whole_t = false)));
-
-        
-//         assert(( forall (whole_t: truth_assignment{ 
-//                     (forall (v : variable_info {(List.Tot.mem v t)}). ((List.Tot.mem v whole_t)))
-//                     /\ are_variables_in_truth_assignment f whole_t 
-//                     /\ length whole_t =  length ( get_vars_in_formula f)}). 
-//                     (is_solution f whole_t = false)) 
-//                 <==> 
-//                 ( forall (whole_t: truth_assignment{ 
-//                     (forall (v : variable_info {(List.Tot.mem v ress)}). ((List.Tot.mem v whole_t)))
-//                     /\ are_variables_in_truth_assignment f whole_t 
-//                     /\ length whole_t =  length ( get_vars_in_formula f)}). 
-//                     (is_solution f whole_t = false)) 
-//                 );
-
-//         assert(L.mem v1 ress);
-
-//         assert(ress = {value = (Var? x) ; variable = (get_literal_variable x)} :: t);
-//         assert(is_variable_in_assignment ress (get_literal_variable x));
-//         assert(is_variable_in_assignment t (get_literal_variable x) = false);
-
-//         assert(forall (l : literal{ is_variable_in_assignment t (get_literal_variable l)}). 
-//                 (is_variable_in_assignment ress (get_literal_variable l)));
-
-//         assert(forall (l : literal{ is_variable_in_assignment ress (get_literal_variable l)
-//             }). 
-//                 (x = (negate_lit l) \/ l = x \/ is_variable_in_assignment t (get_literal_variable l)));
-
-//         assert((forall (l : literal {
-//                 is_variable_in_assignment ress (get_literal_variable l)
-//                 /\ (l <> (negate_lit x))
-//                 /\ (l <> x)}) . 
-//                     (is_variable_in_assignment t (get_literal_variable l))));
-
-//         assert(
-//              is_unit_clause cl res._1 = false);
-//         assert( is_clause_true_yet res._1 cl);
-//         assert( (length res._1 = length t + 1));
-//         assert( (forall (v : variable_info{L.mem v t}). (L.mem v res._1)) );
-//         assert( no_variables_outside_f_are_in_t f res._1);
-//         assert( (( forall (whole_t: truth_assignment{ 
-//                     (forall (v : variable_info {(List.Tot.mem v t)}). ((List.Tot.mem v whole_t)))
-//                     /\ are_variables_in_truth_assignment f whole_t 
-//                     /\ length whole_t =  length ( get_vars_in_formula f)}). 
-//                     (is_solution f whole_t = false)) 
-//                 <==> 
-//                 ( forall (whole_t: truth_assignment{ 
-//                     (forall (v : variable_info {(List.Tot.mem v res._1)}). ((List.Tot.mem v whole_t)))
-//                     /\ are_variables_in_truth_assignment f whole_t 
-//                     /\ length whole_t =  length ( get_vars_in_formula f)}). 
-//                     (is_solution f whole_t = false)) ));
-
-//         assert( is_variable_in_assignment t (get_literal_variable res._2) = false);
-//         assert( is_variable_in_assignment res._1 (get_literal_variable res._2));
-//         assert( is_lit_in_formula f res._2);
-//         assert( (forall (l : literal {
-//                 is_variable_in_assignment res._1 (get_literal_variable l)
-//                 /\ (l <> (negate_lit res._2))
-//                 /\ (l <> res._2)}) . 
-//                     (is_variable_in_assignment t (get_literal_variable l))));
-        
-//         assert( (forall (l : literal {
-//                 is_variable_in_assignment t (get_literal_variable l)
-//             }). (get_literal_value t l = get_literal_value res._1 l)));
-//         ()
-
-
-
 let propagate_unit_clause 
     (f : formula) 
     ( cl : clause{L.mem cl f}) 
@@ -318,19 +118,9 @@ let propagate_unit_clause
         is_unit_clause cl res._1 = false
         /\ is_clause_true_yet res._1 cl
         /\ (length res._1 = length t + 1)
-        /\ (forall (v : variable_info{L.mem v t}). (L.mem v res._1)) 
+        /\ t1_is_sublist_of_t2 t (fst res) 
         /\ no_variables_outside_f_are_in_t f res._1
-        /\ (( forall (whole_t: truth_assignment{ 
-                    (forall (v : variable_info {(List.Tot.mem v t)}). ((List.Tot.mem v whole_t)))
-                    /\ are_variables_in_truth_assignment f whole_t 
-                    /\ length whole_t =  length ( get_vars_in_formula f)}). 
-                    (is_solution f whole_t = false)) 
-                <==> 
-                ( forall (whole_t: truth_assignment{ 
-                    (forall (v : variable_info {(List.Tot.mem v res._1)}). ((List.Tot.mem v whole_t)))
-                    /\ are_variables_in_truth_assignment f whole_t 
-                    /\ length whole_t =  length ( get_vars_in_formula f)}). 
-                    (is_solution f whole_t = false)) )
+        /\ ( (t_cant_be_solution_for_f f t) <==> ( t_cant_be_solution_for_f f (fst res) ))
 
         /\ is_variable_in_assignment t (get_literal_variable res._2) = false
         /\ is_variable_in_assignment res._1 (get_literal_variable res._2)
@@ -349,6 +139,8 @@ let propagate_unit_clause
     let x = get_unassigned_literal_in_unit_clause cl t in
         let x_variable = get_literal_variable x in
         let ress = assign_literal_true_in_truth t x in
+        
+         [@@inline_let]
         let anti_res = assign_literal_true_in_truth t (negate_lit x) in
         assert((length (get_unassigned_literals_from_clause cl t) = 1) /\ (L.hd (get_unassigned_literals_from_clause cl t)) = x);
         assert(forall (n : nat_non_zero{ is_variable_in_assignment t n}). ( is_variable_in_assignment anti_res n));
@@ -368,87 +160,73 @@ let propagate_unit_clause
         assert(is_clause_false_yet anti_res cl = true);
         assert(is_partial_solution f anti_res = false);
 
-        let v1 = {value = Var? (get_unassigned_literal_in_unit_clause cl t) ; variable = (get_literal_variable (get_unassigned_literal_in_unit_clause cl t)) } in
-        let v2 = negate_var_info v1 in
+        [@@inline_let]
+        let v1 =  {value = Var? (get_unassigned_literal_in_unit_clause cl t) ; variable = (get_literal_variable (get_unassigned_literal_in_unit_clause cl t)) } in
+        [@@inline_let]
+        let v2 =  negate_var_info v1 in
 
         assert(
-            forall (other_t : truth_assignment {
-                (forall (v : variable_info{L.mem v anti_res}). (L.mem v other_t))}). 
+            forall (other_t : truth_assignment { t1_is_sublist_of_t2 anti_res other_t}). 
                     (forall (l : literal{L.mem l cl}). (is_variable_in_assignment other_t (get_literal_variable l)))
         );
         assert(
-            forall (other_t : truth_assignment {
-                (forall (v : variable_info{L.mem v anti_res}). (L.mem v other_t))}). 
+            forall (other_t : truth_assignment { t1_is_sublist_of_t2 anti_res other_t}). 
                     (forall (l : literal{L.mem l cl}). (get_literal_value anti_res l = get_literal_value other_t l))
         );
         assert(
-            forall (other_t : truth_assignment {
-                (forall (v : variable_info{L.mem v anti_res}). (L.mem v other_t))}). 
+            forall (other_t : truth_assignment { t1_is_sublist_of_t2 anti_res other_t}). 
                     (get_clause_value anti_res cl = get_clause_value other_t cl)
         );
         assert( get_clause_value anti_res cl = false) ;
         assert(
-            forall (other_t : truth_assignment {
-                (forall (v : variable_info{L.mem v anti_res}). (L.mem v other_t))}). 
+            forall (other_t : truth_assignment { t1_is_sublist_of_t2 anti_res other_t}). 
                     (false = get_clause_value other_t cl)
         );
         assert(
-            forall (other_t : truth_assignment {
-                (forall (v : variable_info{L.mem v anti_res}). (L.mem v other_t))}). 
+            forall (other_t : truth_assignment { t1_is_sublist_of_t2 anti_res other_t}). 
                 (is_partial_solution f other_t = false)
         );
 
         assert(forall (other_t : truth_assignment {
-            (forall (v : variable_info{L.mem v t}). (L.mem v other_t)) 
+            t1_is_sublist_of_t2 t other_t
             /\ L.mem v2 other_t}). (is_partial_solution f other_t = false));
 
         assert(v2 = {value = Var? (negate_lit (get_unassigned_literal_in_unit_clause cl t)) ; variable = (get_literal_variable (get_unassigned_literal_in_unit_clause cl t)) });
         assert(L.mem v2 anti_res);
         assert(( forall (whole_t: truth_assignment{ 
-                (forall (v : variable_info {(List.Tot.mem v t)}). ((List.Tot.mem v whole_t)))
+                t1_is_sublist_of_t2 t whole_t
                 /\ are_variables_in_truth_assignment f whole_t 
                 /\ length whole_t =  length ( get_vars_in_formula f)}). 
                     (is_variable_in_assignment whole_t x_variable)));
 
         assert(( forall (whole_t: truth_assignment{ 
-                (forall (v : variable_info {(List.Tot.mem v t)}). ((List.Tot.mem v whole_t)))
+                t1_is_sublist_of_t2 t whole_t
                 /\ are_variables_in_truth_assignment f whole_t 
                 /\ length whole_t =  length ( get_vars_in_formula f)}). 
                    (L.mem v1 whole_t || L.mem v2 whole_t)));
 
         assert(( forall (whole_t: truth_assignment{ 
-                (forall (v : variable_info {(List.Tot.mem v t)}). ((List.Tot.mem v whole_t)))
+                t1_is_sublist_of_t2 t whole_t
                 /\ are_variables_in_truth_assignment f whole_t 
                 /\ length whole_t =  length ( get_vars_in_formula f)}). 
                    (L.mem v1 whole_t = not (L.mem v2 whole_t))));
 
         assert(( forall (whole_t: truth_assignment{ 
-                (forall (v : variable_info {(List.Tot.mem v t)}). ((List.Tot.mem v whole_t)))
+                t1_is_sublist_of_t2 t whole_t
                 /\ are_variables_in_truth_assignment f whole_t 
                 /\ L.mem v2 whole_t
                 /\ length whole_t =  length ( get_vars_in_formula f)}). 
                    (is_solution f whole_t = false)));
 
         assert(( forall (whole_t: truth_assignment{ 
-                (forall (v : variable_info {(List.Tot.mem v t)}). ((List.Tot.mem v whole_t)))
+                t1_is_sublist_of_t2 t whole_t
                 /\ are_variables_in_truth_assignment f whole_t 
                 /\ (exists (v : variable_info  {L.mem v ress}). (L.mem v whole_t = false))
                 /\ length whole_t =  length ( get_vars_in_formula f)}). 
                    (is_solution f whole_t = false)));
 
         
-        assert(( forall (whole_t: truth_assignment{ 
-                    (forall (v : variable_info {(List.Tot.mem v t)}). ((List.Tot.mem v whole_t)))
-                    /\ are_variables_in_truth_assignment f whole_t 
-                    /\ length whole_t =  length ( get_vars_in_formula f)}). 
-                    (is_solution f whole_t = false)) 
-                <==> 
-                ( forall (whole_t: truth_assignment{ 
-                    (forall (v : variable_info {(List.Tot.mem v ress)}). ((List.Tot.mem v whole_t)))
-                    /\ are_variables_in_truth_assignment f whole_t 
-                    /\ length whole_t =  length ( get_vars_in_formula f)}). 
-                    (is_solution f whole_t = false)) 
-                );
+        assert((t_cant_be_solution_for_f f t) <==> (t_cant_be_solution_for_f f ress ));
 
         assert(L.mem v1 ress);
 
@@ -459,8 +237,7 @@ let propagate_unit_clause
         assert(forall (l : literal{ is_variable_in_assignment t (get_literal_variable l)}). 
                 (is_variable_in_assignment ress (get_literal_variable l)));
 
-        assert(forall (l : literal{ is_variable_in_assignment ress (get_literal_variable l)
-            }). 
+        assert(forall (l : literal{ is_variable_in_assignment ress (get_literal_variable l) }). 
                 (x = (negate_lit l) \/ l = x \/ is_variable_in_assignment t (get_literal_variable l)));
 
         assert((forall (l : literal {
@@ -480,18 +257,8 @@ let rec unit_clause_propagation_helper
     (t : truth_assignment {
         no_variables_outside_f_are_in_t f t 
         /\ length t <= length (get_vars_in_formula f)
-        /\ (forall (v : variable_info{L.mem v original_t}). (L.mem v t))
-        /\ (( forall (whole_t: truth_assignment{ 
-                    (forall (v : variable_info {(List.Tot.mem v t)}). ((List.Tot.mem v whole_t)))
-                    /\ are_variables_in_truth_assignment f whole_t 
-                    /\ length whole_t =  length ( get_vars_in_formula f)}). 
-                    (is_solution f whole_t = false)) 
-                <==> 
-                ( forall (whole_t: truth_assignment{ 
-                    (forall (v : variable_info {(List.Tot.mem v original_t)}). ((List.Tot.mem v whole_t)))
-                    /\ are_variables_in_truth_assignment f whole_t 
-                    /\ length whole_t =  length ( get_vars_in_formula f)}). 
-                    (is_solution f whole_t = false)) )
+        /\ t1_is_sublist_of_t2 original_t t
+        /\ ( (t_cant_be_solution_for_f f t) <==> ( t_cant_be_solution_for_f f original_t ))
     })
     (new_lits : list literal{
         (forall (l : literal {L.mem l new_lits}). 
@@ -512,29 +279,9 @@ let rec unit_clause_propagation_helper
     : Tot (res : (truth_assignment & (list literal))
     {
      no_variables_outside_f_are_in_t f res._1
-    /\ (forall (v :variable_info{L.mem v t}). (L.mem v res._1)) 
-    /\ (( forall (whole_t: truth_assignment{ 
-                    (forall (v : variable_info {(List.Tot.mem v t)}). ((List.Tot.mem v whole_t)))
-                    /\ are_variables_in_truth_assignment f whole_t 
-                    /\ length whole_t =  length ( get_vars_in_formula f)}). 
-                    (is_solution f whole_t = false)) 
-                <==> 
-                ( forall (whole_t: truth_assignment{ 
-                    (forall (v : variable_info {(List.Tot.mem v res._1)}). ((List.Tot.mem v whole_t)))
-                    /\ are_variables_in_truth_assignment f whole_t 
-                    /\ length whole_t =  length ( get_vars_in_formula f)}). 
-                    (is_solution f whole_t = false)) )
-    /\ (( forall (whole_t: truth_assignment{ 
-                    (forall (v : variable_info {(List.Tot.mem v original_t)}). ((List.Tot.mem v whole_t)))
-                    /\ are_variables_in_truth_assignment f whole_t 
-                    /\ length whole_t =  length ( get_vars_in_formula f)}). 
-                    (is_solution f whole_t = false)) 
-                <==> 
-                ( forall (whole_t: truth_assignment{ 
-                    (forall (v : variable_info {(List.Tot.mem v res._1)}). ((List.Tot.mem v whole_t)))
-                    /\ are_variables_in_truth_assignment f whole_t 
-                    /\ length whole_t =  length ( get_vars_in_formula f)}). 
-                    (is_solution f whole_t = false)) )
+    /\ t1_is_sublist_of_t2 t (fst res)
+    /\ ( (t_cant_be_solution_for_f f t) <==> ( t_cant_be_solution_for_f f (fst res) ))
+    /\ ( (t_cant_be_solution_for_f f original_t) <==> ( t_cant_be_solution_for_f f (fst res) ))
     /\ length res._1 >= length t
     /\ (forall (l : literal {L.mem l res._2}). 
         (
@@ -634,7 +381,9 @@ let rec unit_clause_propagation_helper
         assert(forall (l : literal{L.mem l new_lits_2}). (L.mem l new_lits \/ l = new_t._2 ));
 
         assert(forall (l : literal{L.mem l new_lits}). (L.mem l new_lits_2));
+         [@@inline_let]
         let negated_new_lits = negate_lits_list new_lits in
+         [@@inline_let]
         let negated_new_lits_2 = negate_lits_list new_lits_2 in
         
         assert(forall (l : literal{L.mem l new_lits}). 
@@ -721,7 +470,6 @@ let rec unit_clause_propagation_helper
         (
             is_variable_in_assignment ress._1 (get_literal_variable l)
             /\ (is_variable_in_assignment (L.tl original_t) (get_literal_variable l) = false)
-            //\ is_lit_in_formula f l
         )));
 
         assert((forall (l : literal{L.mem l ress._2}). 
@@ -788,18 +536,8 @@ let unit_clause_propagation
     : Tot (res : (truth_assignment & (list literal))
     {
      no_variables_outside_f_are_in_t f res._1
-    /\ (forall (v :variable_info{L.mem v t}). (L.mem v res._1)) 
-    /\ (( forall (whole_t: truth_assignment{ 
-                    (forall (v : variable_info {(List.Tot.mem v t)}). ((List.Tot.mem v whole_t)))
-                    /\ are_variables_in_truth_assignment f whole_t 
-                    /\ length whole_t =  length ( get_vars_in_formula f)}). 
-                    (is_solution f whole_t = false)) 
-                <==> 
-                ( forall (whole_t: truth_assignment{ 
-                    (forall (v : variable_info {(List.Tot.mem v res._1)}). ((List.Tot.mem v whole_t)))
-                    /\ are_variables_in_truth_assignment f whole_t 
-                    /\ length whole_t =  length ( get_vars_in_formula f)}). 
-                    (is_solution f whole_t = false)) )
+    /\ t1_is_sublist_of_t2 t (fst res)
+    /\ ((t_cant_be_solution_for_f f t) <==> ( t_cant_be_solution_for_f f (fst res)) )
     /\ length res._1 >= length t
     /\ (forall (l : literal {L.mem l res._2}). 
         (
@@ -840,7 +578,6 @@ let unit_clause_propagation
         
         let ress = unit_clause_propagation_helper f t t new_lits in
         assert(forall (l : literal {L.mem l new_lits}). (L.mem l ress._2));
-        assert( (L.mem new_l ress._2)
-                );
+        assert( L.mem new_l ress._2 );
 
         ress
