dpll_optimized/ConvertorToString.fst
@@ -1,0 +1,97 @@
+module ConvertorToString 
+
+open FStar.String
+open FStar.List.Tot
+
+module L = FStar.List.Tot
+
+open DataTypes
+
+let new_line_string = "\n"
+
+let concat_to_truth (s1 : string) (s2 : string) = concat new_line_string [s1 ; s2]
+
+
+let rec int_to_string (i : nat) =
+    if i = 0
+    then "0"
+    else 
+        if i > 9
+        then    
+            let last_digit = i `op_Modulus` 10 in
+            let other_digits = i `op_Division` 10 in
+            let res = concat "" [(int_to_string other_digits) ; (int_to_string last_digit)] in
+            res
+        else
+            if i = 1
+            then "1"
+            else
+            if i = 2
+            then "2"
+            else
+            if i = 3
+            then "3"
+            else
+            if i = 4
+            then "4"
+            else
+            if i = 5
+            then "5"
+            else
+            if i = 6
+            then "6"
+            else
+            if i = 7
+            then "7"
+            else
+            if i = 8
+            then "8"
+            else "9"
+
+let bool_to_string (b : bool) =
+    if b 
+    then "True"
+    else "False"
+
+let literal_to_string (l : literal) =
+    match l with
+    | Var x -> int_to_string x
+    | NotVar x -> concat "" [ "-" ; int_to_string x]
+
+let rec clause_to_string (c : clause) =
+    let x = L.hd c in
+    let x_str = literal_to_string x in
+        if length c = 1
+        then x_str
+        else
+            let xs_str = clause_to_string (L.tl c) in
+            concat "  /\\  " [x_str ; xs_str]
+
+let rec formula_to_string (f : formula{length f > 0}) : (res : string)
+    = 
+    let x = L.hd f in
+    let x_str = clause_to_string x in
+        if length f = 1
+        then x_str
+        else
+            let xs_str = formula_to_string (L.tl f) in
+            concat "\n" [x_str ; xs_str]
+
+
+
+let var_info_to_string (v : variable_info) : (res : string)
+    = 
+    let var_string = int_to_string v.variable in
+    let var_value = bool_to_string v.value in
+    concat " = " [var_string ; var_value]
+
+let rec truth_to_string (t : truth_assignment {length t > 0}) : (t_string : string) =
+    let x = L.hd t in
+    let x_to_string = var_info_to_string x in
+        if length t = 1
+        then concat_to_truth x_to_string "\nSatisfiable"
+        else
+            let xs = L.tl t in
+            let xs_to_string = truth_to_string xs in
+            let res = concat_to_truth x_to_string xs_to_string in
+            res 
