dpll_optimized/Main.fst
@@ -1,25 +1,29 @@
 module Main
 
 open DataTypes
+open DataTypeUtils
 open Dpll
 open InputFileParser
-open FStar.IO
-open FStar.List.Tot
+open ConvertorToString
 
 open FStar.IO
+open FStar.List.Tot
+open FStar.String
 
 let main = 
     let file_name = input_line () in
     let input_formula = getInput file_name in
-    if (length input_formula = 0)
+    if (FStar.List.Tot.length input_formula = 0)
     then 
         print_string "formula has length 0"
     else 
         let res = dpll input_formula in
-            if Sat? res = true
+        let formula_str = formula_to_string input_formula in
+            if Sat? res 
             then 
-                let mess = "True" in
-                print_string mess
+                let truth_str = truth_to_string (get_truth_from_result res) in 
+                let formula_truth_to_str = truth_str in// concat "\n\n" [formula_str ; truth_str] in
+                print_string formula_truth_to_str
             else 
-                let mess = "False" in 
-                print_string mess
+                let str_res = "Unsatisfiable" in // concat "\n" [formula_str ; "Unsatisfiable"] in
+                print_string str_res
